BatchOpening binding proof structure complete

KZG_BatchOpening_binding.thy
@@ -15,6 +15,9 @@ definition key_gen:: "'a pk spmf" where
 
 definition valid_msg :: "'e eval_value \<Rightarrow> 'a eval_witness \<Rightarrow> bool" where 
   "valid_msg \<phi>_i w_i = (w_i \<in> carrier G\<^sub>p)"
+
+definition valid_batch_msg :: "'e polynomial \<Rightarrow> 'a eval_witness \<Rightarrow> 'e eval_position set \<Rightarrow> bool" where 
+  "valid_batch_msg r_x w_B B = (w_B \<in> carrier G\<^sub>p \<and> degree r_x < card B)"
                     
 subsection \<open>Game definition\<close>
 
@@ -27,7 +30,7 @@ definition bind_game :: "('a, 'e) adversary \<Rightarrow> bool spmf"
   where "bind_game \<A> = TRY do {
   PK \<leftarrow> key_gen;
   (C, i, \<phi>_i, w_i, B, w_B, r_x) \<leftarrow> \<A> PK;
-  _ :: unit \<leftarrow> assert_spmf (i \<in> B \<and> \<phi>_i \<noteq> poly r_x i \<and> valid_msg \<phi>_i w_i); 
+  _ :: unit \<leftarrow> assert_spmf (card B < max_deg \<and> i \<in> B \<and> \<phi>_i \<noteq> poly r_x i \<and> valid_msg \<phi>_i w_i \<and> valid_batch_msg r_x w_B B); 
   let b = VerifyEval PK C i \<phi>_i w_i;
   let b' = VerifyEvalBatch PK C B r_x w_B;
   return_spmf (b \<and> b')} ELSE return_spmf False"
@@ -48,21 +51,149 @@ fun bind_reduction
 where
   "bind_reduction \<A> PK = do {
    (C, i, \<phi>_i, w_i, B, w_B, r_x) \<leftarrow> \<A> PK;
-  _ :: unit \<leftarrow> assert_spmf (i \<in> B \<and> \<phi>_i \<noteq> poly r_x i \<and> valid_msg \<phi>_i w_i
+  _ :: unit \<leftarrow> assert_spmf (card B < max_deg \<and> i \<in> B \<and> \<phi>_i \<noteq> poly r_x i \<and> valid_msg \<phi>_i w_i \<and> valid_batch_msg r_x w_B B
                             \<and> VerifyEval PK C i \<phi>_i w_i \<and> VerifyEvalBatch PK C B r_x w_B);
   let p' = g_pow_PK_Prod PK (prod (\<lambda>i. [:-i,1:]) B div [:-i,1:]);
   let r' = g_pow_PK_Prod PK ((r_x - [:poly r_x i:]) div [:-i,1:]);
   return_spmf (-i::'e mod_ring, e p' w_B \<otimes>\<^bsub>G\<^sub>T\<^esub> e (r' \<div>\<^bsub>G\<^sub>p\<^esub> w_i) \<^bold>g ^\<^bsub>G\<^sub>T\<^esub> (1/(\<phi>_i - poly r_x i))) }"
+
+text \<open>An alternative but equivalent game for the binding game. 
+This alternative game capsulates the 
+event that the Adversary wins in the assert_spmf statement.
+It's a closely adapted proof from Sigma_Commit_Crypto.Commitment_Schemes bind_game_alt_def\<close>
+lemma bind_game_alt_def:
+  "bind_game \<A> = TRY do {
+  PK \<leftarrow> key_gen;
+  (C, i, \<phi>_i, w_i, B, w_B, r_x) \<leftarrow> \<A> PK;
+  _ :: unit \<leftarrow> assert_spmf (card B < max_deg \<and> i \<in> B \<and> \<phi>_i \<noteq> poly r_x i \<and> valid_msg \<phi>_i w_i \<and> valid_batch_msg r_x w_B B); 
+  let b = VerifyEval PK C i \<phi>_i w_i;
+  let b' = VerifyEvalBatch PK C B r_x w_B;
+  _::unit \<leftarrow> assert_spmf (b \<and> b');
+  return_spmf True} ELSE return_spmf False"
+  (is "?lhs = ?rhs")
+proof -
+  have "?lhs = TRY do {
+    PK \<leftarrow> key_gen;
+    TRY do {
+    (C, i, \<phi>_i, w_i, B, w_B, r_x) \<leftarrow> \<A> PK;
+    TRY do {
+    _ :: unit \<leftarrow> assert_spmf (card B < max_deg \<and> i \<in> B \<and> \<phi>_i \<noteq> poly r_x i \<and> valid_msg \<phi>_i w_i \<and> valid_batch_msg r_x w_B B); 
+    TRY do {
+    let b = VerifyEval PK C i \<phi>_i w_i;
+    let b' = VerifyEvalBatch PK C B r_x w_B;
+    return_spmf (b \<and> b')
+    } ELSE return_spmf False
+    } ELSE return_spmf False
+    } ELSE return_spmf False
+  } ELSE return_spmf False"
+    unfolding split_def bind_game_def
+    by(fold try_bind_spmf_lossless2[OF lossless_return_spmf]) simp
+  also have "\<dots> = TRY do {
+    PK \<leftarrow> key_gen;
+    TRY do {
+    (C, i, \<phi>_i, w_i, B, w_B, r_x) \<leftarrow> \<A> PK;
+    TRY do {
+    _ :: unit \<leftarrow> assert_spmf (card B < max_deg \<and> i \<in> B \<and> \<phi>_i \<noteq> poly r_x i \<and> valid_msg \<phi>_i w_i \<and> valid_batch_msg r_x w_B B); 
+    TRY do {
+    let b = VerifyEval PK C i \<phi>_i w_i;
+    let b' = VerifyEvalBatch PK C B r_x w_B;
+    _::unit \<leftarrow> assert_spmf (b \<and> b');
+    return_spmf True
+    } ELSE return_spmf False
+    } ELSE return_spmf False
+    } ELSE return_spmf False
+  } ELSE return_spmf False"   
+    by(auto simp add: try_bind_assert_spmf try_spmf_return_spmf1 intro!: try_spmf_cong bind_spmf_cong)
+  also have "\<dots> = ?rhs"
+    unfolding split_def Let_def
+    by(fold try_bind_spmf_lossless2[OF lossless_return_spmf]) simp
+  finally show ?thesis .
+qed
 
 end
 
 locale bind_game_proof = bind_game_def
 begin
 
+lemma assert_anding: "TRY do {
+          _ :: unit \<leftarrow> assert_spmf (a);
+            _ :: unit \<leftarrow> assert_spmf (b);
+            return_spmf True
+        } ELSE return_spmf False 
+    = TRY do {
+          _ :: unit \<leftarrow> assert_spmf (a \<and> b);
+          return_spmf True
+      } ELSE return_spmf False"
+  by (simp add: try_bind_assert_spmf) 
+
+lemma verifys_impl_t_BSDH_break: 
+  assumes 
+    "card B < max_deg \<and> i \<in> B \<and>  \<phi>_i \<noteq> poly r_x i \<and> valid_msg \<phi>_i w_i \<and> valid_batch_msg r_x w_B B \<and>
+    VerifyEval (map (\<lambda>t. \<^bold>g ^ \<alpha> ^ t) [0..<max_deg + 1]) C i \<phi>_i w_i \<and>
+    VerifyEvalBatch (map (\<lambda>t. \<^bold>g ^ \<alpha> ^ t) [0..<max_deg + 1]) C B r_x
+                     w_B"
+  shows " e \<^bold>g \<^bold>g ^\<^bsub>G\<^sub>T\<^esub> (1 / (\<alpha> + - i))
+        =
+          e (g_pow_PK_Prod (map (\<lambda>t. \<^bold>g ^ \<alpha> ^ t) [0..<max_deg + 1])
+              ((\<Prod>i\<in>B. [:- i, 1:]) div [:- i, 1:]))
+           w_B 
+        \<otimes>\<^bsub>G\<^sub>T\<^esub>
+          e (g_pow_PK_Prod (map (\<lambda>t. \<^bold>g ^ \<alpha> ^ t) [0..<max_deg + 1])
+              ((r_x - [:poly r_x i:]) div [:- i, 1:]) \<otimes>
+             inv w_i)
+           \<^bold>g ^\<^bsub>G\<^sub>T\<^esub>
+          (1 / (\<phi>_i - poly r_x i))"
+proof -
+  obtain b where b: "w_B = \<^bold>g ^ b"
+    using assms unfolding valid_batch_msg_def
+    by (metis G\<^sub>p.generatorE g_pow_to_int_mod_ring_of_int_mod_ring int_pow_int)
+  obtain y where y: "w_i = \<^bold>g ^ y"
+    using assms unfolding valid_msg_def
+    by (metis G\<^sub>p.generatorE g_pow_to_int_mod_ring_of_int_mod_ring int_pow_int)
+
+  from assms have "e w_i (map (\<lambda>t. \<^bold>g ^ \<alpha> ^ t) [0..<max_deg + 1] ! 1 \<otimes> inv (\<^bold>g ^ i)) \<otimes>\<^bsub>G\<^sub>T\<^esub> e \<^bold>g \<^bold>g ^\<^bsub>G\<^sub>T\<^esub> \<phi>_i
+    = e (g_pow_PK_Prod (map (\<lambda>t. \<^bold>g ^ \<alpha> ^ t) [0..<max_deg + 1]) (\<Prod>i\<in>B. [:- i, 1:])) w_B \<otimes>\<^bsub>G\<^sub>T\<^esub>
+  e \<^bold>g (g_pow_PK_Prod (map (\<lambda>t. \<^bold>g ^ \<alpha> ^ t) [0..<max_deg + 1]) r_x)" (is "?lhs = ?rhs")
+    unfolding VerifyEval_def VerifyEvalBatch_def Let_def by presburger
+  moreover have "?lhs = e (\<^bold>g ^ y) (\<^bold>g ^ (\<alpha>-i) ) \<otimes>\<^bsub>G\<^sub>T\<^esub> e \<^bold>g \<^bold>g ^\<^bsub>G\<^sub>T\<^esub> \<phi>_i"
+    unfolding y using PK_i d_pos mod_ring_pow_mult_inv_G\<^sub>p by auto
+  moreover have "?rhs = e (\<^bold>g ^ poly (\<Prod>i\<in>B. [:- i, 1:]) \<alpha>) (\<^bold>g ^ b) \<otimes>\<^bsub>G\<^sub>T\<^esub> e \<^bold>g (\<^bold>g ^ poly r_x \<alpha>)"
+    using g_pow_PK_Prod_correct sorry
+  show ?thesis
+    using assms unfolding VerifyEval_def VerifyEvalBatch_def Let_def
+    
+    sorry
+qed
+
+lemma literal_helping: 
+  "(card B < max_deg \<and> i \<in> (B::'e eval_position set) \<and>
+                    (\<phi>_i:: 'e eval_value) \<noteq> (poly r_x i:: 'e eval_value) \<and>
+                    valid_msg \<phi>_i w_i \<and> valid_batch_msg r_x w_B B \<and> 
+                    VerifyEval (map (\<lambda>t. \<^bold>g\<^bsub>G\<^sub>p\<^esub> ^\<^bsub>G\<^sub>p\<^esub> \<alpha> ^ t) [0..<max_deg + 1]) C i \<phi>_i w_i \<and>
+                    VerifyEvalBatch (map (\<lambda>t. \<^bold>g\<^bsub>G\<^sub>p\<^esub> ^\<^bsub>G\<^sub>p\<^esub> (\<alpha>::'e mod_ring) ^ t) [0..<max_deg + 1]) C B r_x w_B \<and>
+                    e \<^bold>g \<^bold>g ^\<^bsub>G\<^sub>T\<^esub> (1 / (\<alpha> + - i)) =
+                    e (g_pow_PK_Prod (map (\<lambda>t. \<^bold>g\<^bsub>G\<^sub>p\<^esub> ^\<^bsub>G\<^sub>p\<^esub> \<alpha> ^ t) [0..<max_deg + 1])
+                        ((\<Prod>i\<in>B. [:- i, 1:]) div [:- i, 1:]))
+                     w_B \<otimes>\<^bsub>G\<^sub>T\<^esub>
+                    e (g_pow_PK_Prod (map (\<lambda>t. \<^bold>g\<^bsub>G\<^sub>p\<^esub> ^\<^bsub>G\<^sub>p\<^esub> \<alpha> ^ t) [0..<max_deg + 1])
+                        ((r_x - [:poly r_x i:]) div [:- i, 1:]) \<otimes>
+                       inv w_i)
+                     \<^bold>g ^\<^bsub>G\<^sub>T\<^esub>
+                    ((1::'e mod_ring) / (\<phi>_i - poly r_x i)))
+  \<longleftrightarrow>
+  (card B < max_deg \<and> i \<in> B \<and>
+                    \<phi>_i \<noteq> poly r_x i \<and> 
+                    valid_msg \<phi>_i w_i \<and> valid_batch_msg r_x w_B B \<and>
+                    VerifyEval (map (\<lambda>t. \<^bold>g\<^bsub>G\<^sub>p\<^esub> ^\<^bsub>G\<^sub>p\<^esub> \<alpha> ^ t) [0..<max_deg + 1]) C i \<phi>_i w_i \<and>
+                    VerifyEvalBatch (map (\<lambda>t. \<^bold>g\<^bsub>G\<^sub>p\<^esub> ^\<^bsub>G\<^sub>p\<^esub> \<alpha> ^ t) [0..<max_deg + 1]) C B r_x
+                     w_B)"
+  using verifys_impl_t_BSDH_break by fast
+
+
 theorem bind_game_eq_t_BSDH_red:
   shows "bind_game \<A> = t_BSDH.game (bind_reduction \<A>)"
 proof - 
-    note [simp] = Let_def split_def
+  note [simp] = Let_def split_def
 
   text \<open>abbreviations for the mod_ring version of sample uniform nat 
   and the public key\<close>
@@ -78,21 +209,21 @@ proof -
   also have "\<dots> = TRY do { 
     \<alpha> \<leftarrow> sample_uniform (order G\<^sub>p);
     (C, i, \<phi>_i, w_i, B, w_B, r_x) \<leftarrow> \<A> (?PK \<alpha>);
-    _ :: unit \<leftarrow> assert_spmf (i \<in> B \<and> \<phi>_i \<noteq> poly r_x i \<and> valid_msg \<phi>_i w_i
+    _ :: unit \<leftarrow> assert_spmf (card B < max_deg \<and> i \<in> B \<and> \<phi>_i \<noteq> poly r_x i \<and> valid_msg \<phi>_i w_i \<and> valid_batch_msg r_x w_B B
                               \<and> VerifyEval (?PK \<alpha>) C i \<phi>_i w_i \<and> VerifyEvalBatch (?PK \<alpha>) C B r_x w_B);
     let p' = g_pow_PK_Prod (?PK \<alpha>) (prod (\<lambda>i. [:-i,1:]) B div [:-i,1:]);
     let r' = g_pow_PK_Prod (?PK \<alpha>) ((r_x - [:poly r_x i:]) div [:-i,1:]);
     _::unit \<leftarrow>  assert_spmf ((e \<^bold>g \<^bold>g) ^\<^bsub>G\<^sub>T\<^esub> (1/((?mr \<alpha>)+(-i))) = e p' w_B \<otimes>\<^bsub>G\<^sub>T\<^esub> e (r' \<div>\<^bsub>G\<^sub>p\<^esub> w_i) \<^bold>g ^\<^bsub>G\<^sub>T\<^esub> (1/(\<phi>_i - poly r_x i))); 
     return_spmf True  
   } ELSE return_spmf False"
-    by simp
+    by force
   text \<open>fold the two asserts together so we can reason about their joined content.\<close>
   also have "\<dots> = TRY do { 
     \<alpha> \<leftarrow> sample_uniform (order G\<^sub>p);
     TRY do {
     (C, i, \<phi>_i, w_i, B, w_B, r_x) \<leftarrow> \<A> (?PK \<alpha>);
     TRY do {
-    _ :: unit \<leftarrow> assert_spmf (i \<in> B \<and> \<phi>_i \<noteq> poly r_x i \<and> valid_msg \<phi>_i w_i
+    _ :: unit \<leftarrow> assert_spmf (card B < max_deg \<and> i \<in> B \<and> \<phi>_i \<noteq> poly r_x i \<and> valid_msg \<phi>_i w_i \<and> valid_batch_msg r_x w_B B
                               \<and> VerifyEval (?PK \<alpha>) C i \<phi>_i w_i \<and> VerifyEvalBatch (?PK \<alpha>) C B r_x w_B);
     let p' = g_pow_PK_Prod (?PK \<alpha>) (prod (\<lambda>i. [:-i,1:]) B div [:-i,1:]);
     let r' = g_pow_PK_Prod (?PK \<alpha>) ((r_x - [:poly r_x i:]) div [:-i,1:]);
@@ -110,7 +241,7 @@ proof -
     TRY do {
      let p' = g_pow_PK_Prod (?PK \<alpha>) (prod (\<lambda>i. [:-i,1:]) B div [:-i,1:]);
     let r' = g_pow_PK_Prod (?PK \<alpha>) ((r_x - [:poly r_x i:]) div [:-i,1:]);
-    _ :: unit \<leftarrow> assert_spmf (i \<in> B \<and> \<phi>_i \<noteq> poly r_x i \<and> valid_msg \<phi>_i w_i
+    _ :: unit \<leftarrow> assert_spmf (card B < max_deg \<and> i \<in> B \<and> \<phi>_i \<noteq> poly r_x i \<and> valid_msg \<phi>_i w_i \<and> valid_batch_msg r_x w_B B
                               \<and> VerifyEval (?PK \<alpha>) C i \<phi>_i w_i \<and> VerifyEvalBatch (?PK \<alpha>) C B r_x w_B
                               \<and> (e \<^bold>g \<^bold>g) ^\<^bsub>G\<^sub>T\<^esub> (1/((?mr \<alpha>)+(-i))) 
                                 = e p' w_B \<otimes>\<^bsub>G\<^sub>T\<^esub> e (r' \<div>\<^bsub>G\<^sub>p\<^esub> w_i) \<^bold>g ^\<^bsub>G\<^sub>T\<^esub> (1/(\<phi>_i - poly r_x i))); 
@@ -118,11 +249,65 @@ proof -
     } ELSE return_spmf False
     } ELSE return_spmf False
   } ELSE return_spmf False"
-    sorry 
-
-  show ?thesis 
-    sorry
-
+    using assert_anding by algebra
+    also have "\<dots> = TRY do { 
+    \<alpha> \<leftarrow> sample_uniform (order G\<^sub>p);
+    (C, i, \<phi>_i, w_i, B, w_B, r_x) \<leftarrow> \<A> (?PK \<alpha>);
+    let p' = g_pow_PK_Prod (?PK \<alpha>) (prod (\<lambda>i. [:-i,1:]) B div [:-i,1:]);
+    let r' = g_pow_PK_Prod (?PK \<alpha>) ((r_x - [:poly r_x i:]) div [:-i,1:]);
+    _ :: unit \<leftarrow> assert_spmf (card B < max_deg \<and> i \<in> B \<and> \<phi>_i \<noteq> poly r_x i \<and> valid_msg \<phi>_i w_i \<and> valid_batch_msg r_x w_B B
+                              \<and> VerifyEval (?PK \<alpha>) C i \<phi>_i w_i \<and> VerifyEvalBatch (?PK \<alpha>) C B r_x w_B
+                              \<and> (e \<^bold>g \<^bold>g) ^\<^bsub>G\<^sub>T\<^esub> (1/((?mr \<alpha>)+(-i))) 
+                                = e p' w_B \<otimes>\<^bsub>G\<^sub>T\<^esub> e (r' \<div>\<^bsub>G\<^sub>p\<^esub> w_i) \<^bold>g ^\<^bsub>G\<^sub>T\<^esub> (1/(\<phi>_i - poly r_x i))); 
+    return_spmf True  
+  } ELSE return_spmf False"
+   unfolding split_def Let_def
+   by(fold try_bind_spmf_lossless2[OF lossless_return_spmf]) simp
+  also have "\<dots> = TRY do { 
+    \<alpha> \<leftarrow> sample_uniform (order G\<^sub>p);
+    (C, i, \<phi>_i, w_i, B, w_B, r_x) \<leftarrow> \<A> (?PK \<alpha>);
+    _ :: unit \<leftarrow> assert_spmf (card B < max_deg \<and> i \<in> B \<and> \<phi>_i \<noteq> poly r_x i \<and> valid_msg \<phi>_i w_i \<and> valid_batch_msg r_x w_B B
+                              \<and> VerifyEval (?PK \<alpha>) C i \<phi>_i w_i \<and> VerifyEvalBatch (?PK \<alpha>) C B r_x w_B); 
+    return_spmf True  
+  } ELSE return_spmf False"
+    unfolding Let_def using literal_helping by algebra 
+  also have "\<dots> = TRY do { 
+    \<alpha> \<leftarrow> sample_uniform (order G\<^sub>p);
+    TRY do {
+    (C, i, \<phi>_i, w_i, B, w_B, r_x) \<leftarrow> \<A> (?PK \<alpha>);
+    TRY do {
+    _ :: unit \<leftarrow> assert_spmf (card B < max_deg \<and> i \<in> B \<and> \<phi>_i \<noteq> poly r_x i \<and> valid_msg \<phi>_i w_i \<and> valid_batch_msg r_x w_B B
+                              \<and> VerifyEval (?PK \<alpha>) C i \<phi>_i w_i \<and> VerifyEvalBatch (?PK \<alpha>) C B r_x w_B); 
+    return_spmf True  
+     } ELSE return_spmf False
+    } ELSE return_spmf False
+  } ELSE return_spmf False"
+  unfolding split_def Let_def
+  by(fold try_bind_spmf_lossless2[OF lossless_return_spmf]) simp
+  also have "\<dots> = TRY do { 
+    \<alpha> \<leftarrow> sample_uniform (order G\<^sub>p);
+    TRY do {
+    (C, i, \<phi>_i, w_i, B, w_B, r_x) \<leftarrow> \<A> (?PK \<alpha>);
+    TRY do {
+    _ :: unit \<leftarrow> assert_spmf (card B < max_deg \<and> i \<in> B \<and> \<phi>_i \<noteq> poly r_x i \<and> valid_msg \<phi>_i w_i \<and> valid_batch_msg r_x w_B B);
+    _ :: unit \<leftarrow> assert_spmf (VerifyEval (?PK \<alpha>) C i \<phi>_i w_i \<and> VerifyEvalBatch (?PK \<alpha>) C B r_x w_B); 
+    return_spmf True  
+     } ELSE return_spmf False
+    } ELSE return_spmf False
+  } ELSE return_spmf False" 
+    using assert_anding by algebra
+  also have "\<dots> = TRY do { 
+    \<alpha> \<leftarrow> sample_uniform (order G\<^sub>p);
+    (C, i, \<phi>_i, w_i, B, w_B, r_x) \<leftarrow> \<A> (?PK \<alpha>);
+    _ :: unit \<leftarrow> assert_spmf (card B < max_deg \<and> i \<in> B \<and> \<phi>_i \<noteq> poly r_x i \<and> valid_msg \<phi>_i w_i \<and> valid_batch_msg r_x w_B B);
+    _ :: unit \<leftarrow> assert_spmf (VerifyEval (?PK \<alpha>) C i \<phi>_i w_i \<and> VerifyEvalBatch (?PK \<alpha>) C B r_x w_B); 
+    return_spmf True
+  } ELSE return_spmf False" 
+  unfolding split_def Let_def
+  by(fold try_bind_spmf_lossless2[OF lossless_return_spmf]) simp
+  also have "\<dots>= bind_game \<A>"
+    using bind_game_alt_def unfolding key_gen_def Setup_def by simp
+  finally show ?thesis ..
 qed
 
 theorem batchOpening_binding: "bind_advantage \<A> = t_BSDH.advantage (bind_reduction \<A>)"
